\documentclass[12pt]{article}

\usepackage[utf8]{inputenc}
\usepackage{latexsym,amsfonts,amssymb,amsthm,amsmath}

\setlength{\parindent}{0in}
\setlength{\oddsidemargin}{0in}
\setlength{\textwidth}{6.5in}
\setlength{\textheight}{8.8in}
\setlength{\topmargin}{0in}
\setlength{\headheight}{18pt}



\title{Homework 5}
\author{N. Ohayon Rozanes}

\begin{document}

\maketitle

\vspace{0.5in}



\subsection*{Exercise 1}
\begin{enumerate}
  \item $H_0 = \beta_1 + 2\beta_2 = 3$ 
    \begin{align*}
      \mathbf{D} = \begin{bmatrix}
      1 & 2 & 0 & 0
    \end{bmatrix} 
    \quad 
    \mathbf{d} = \begin{bmatrix}
     3 
    \end{bmatrix}
    \end{align*}
  \item $H_0: \frac{\beta_1 + \beta_2}{2} = \beta_3 \implies H_0: \frac{\beta_1 + \beta_2}{2} - \beta_3 = 0$ 

  \[
      \mathbf{d} = \begin{bmatrix}
      \frac12 & \frac12 & -1 & 0
    \end{bmatrix} 
    \quad 
    \mathbf{d} = \begin{bmatrix}
     0 
    \end{bmatrix}
  \]
\item $H_0: \beta_1  = \beta_2, \beta_3 = \beta_4 \implies \beta_1 - \beta_2 = 0, \beta_3- \beta_4$ 
  \[
    \mathbf{d} = \begin{bmatrix}
      1 & -1 &0&0  \\
      0 & 0 & 1 & - 1
    \end{bmatrix} 
    \quad 
    \mathbf{d} = \begin{bmatrix}
     0 \\ 
     0
    \end{bmatrix}
  \]
\item $H_0: \beta_1 - 2\beta_2 - 4\beta_3 = 0, \beta_1 + 2\beta_2 = 0$
\[
    \mathbf{d} = \begin{bmatrix}
      1 & -2 &-4&0  \\
      1& 2 & 0 &0
    \end{bmatrix} 
    \quad 
    \mathbf{d} = \begin{bmatrix}
     0 \\ 
     0
    \end{bmatrix}
\]
\item $H_0: \beta_1 -\beta_2 = 0, \beta_2 - \beta_3 = 0, \beta_3 - \beta_4 = 0$
\[
    \mathbf{d} = \begin{bmatrix}
      1 & -1 &0&0  \\
      0& 1 & -1 &0 \\ 
      0& 0& 1& -1 \\
    \end{bmatrix} 
    \quad 
    \mathbf{d} = \begin{bmatrix}
     0 \\ 
     0 \\ 
     0
    \end{bmatrix}
\]
\end{enumerate}
\end{document}

