\documentclass[12pt]{article}

\usepackage[utf8]{inputenc}
\usepackage{latexsym,amsfonts,amssymb,amsthm,amsmath}

\setlength{\parindent}{0in}
\setlength{\oddsidemargin}{0in}
\setlength{\textwidth}{6.5in}
\setlength{\textheight}{8.8in}
\setlength{\topmargin}{0in}
\setlength{\headheight}{18pt}



\title{Homework 4}
\author{N. Ohayon Rozanes}

\begin{document}

\maketitle

\vspace{0.5in}



\subsection*{Exercise 1}
\begin{proof}
  multiplying out the terms and simplifying we get that
  \begin{align*}
    (I - H)(I - H) &= I - 2H + HH 
  \end{align*}
  However, since $H$ is a project matrix and therefore idempotent, we can say that $HH = H$ so: 
  \begin{align*}
    I - 2H + HH &= I - 2H + H\\
                &= I - H
  \end{align*}
  Thererfore we have proven that $(I - H)^2 = (I - H)$ is idempotent
\end{proof}
\subsection*{Exercise 2}
\begin{proof}
  Clearly
  \begin{align*}
    Var(Ay) &= E[Ay - E(Ay)](Ay - E[Ay]))' \\
            &= E[A(y - E(y))](A(y - E[y])) \\
            &= AE[(y - E(y))](y - E[y]))'A' \\
            &= AVar(y)A' \\
  \end{align*}
\end{proof}
\subsection*{Exercise 3}
\begin{enumerate}
  \item 
\begin{proof}
\end{proof}
\end{enumerate}
\end{document}

